
	\documentclass{article}
	\usepackage{amsmath,amssymb}
	\usepackage[inline]{enumitem}
	\usepackage{blindtext}
	\usepackage{booktabs}
	\usepackage{graphicx}
	\usepackage{xcolor}
	\usepackage[vmargin = 1.5in, top = 1in, bottom = 1.2in, letterpaper]{geometry}
	\usepackage{listings}
	\usepackage{courier}
	\usepackage{multicol}
	\usepackage{multirow}
	\usepackage{bm}
	\lstset{
	basicstyle = \small\tt,
	keywordstyle = \tt\color{blue},
	commentstyle = \it\color[cmyk]{1,0,1,0},
	stringstyle = \tt\color[RGB]{128,0,0},
	%frame = single,
	backgroundcolor = \color[RGB]{245,245,244},
	breaklines,
	extendedchars = false,
	xleftmargin = 2em,
	xrightmargin = 2em,
	aboveskip = 1em,
	tabsize = 4,
	showspaces = false
	}
	\begin{document}
	
	% \newfontfamily\courier{Courier New}

	
	\title{STAT 543 Homework 1}
	\author{Yifan Zhu}
	\maketitle
	
	\begin{enumerate}[leftmargin = 0 em, label = \arabic*., font = \bfseries]
	\item 
	\begin{enumerate}
		\item 
		\[\mu_1' = E(X) \Rightarrow \mu_1 ' = \frac{3(1 - p)}{p}\]
		Hence
		\[p \mu_1 ' = 3(1 - p) \Rightarrow p = \frac{3}{\mu_1 ' + 3} = \frac{3}{\frac{\sum_{i=1}^n X_i}{n} + 3}\]

		\item 
		\begin{align*}
		& \mu_1 '  = E(X) = \mu\\
		& \mu_2' = E(X^2) = (E(X))^2 + Var(X) = \mu^2 + 2 \sigma^2
		\end{align*}
		Hence
		\begin{align*}
		& \mu = \mu_1' = \frac{\sum_{i=1}^n X_i}{n}\\
		& \sigma = \sqrt{\frac{\mu_2' - \mu_1'^2}{2}} = \sqrt{\frac{\sum_{i=1}^n X_i^2}{2n} - \frac{(\sum_{i=1}^n X_i)^2}{2 n^2}}
		\end{align*}
		
		
	\end{enumerate}

	\item 
	For a given $x$, $\hat{\theta}$ maximize $f(x|\theta)$, thus

	When $x = 0$, $\hat{\theta} = 1$.

	When $x = 1$, $\hat{\theta} = 1$.

	When $x = 2$, $\hat{\theta} = 2,3$.

	When $x = 3$, $\hat{\theta} = 3$.

	When $x = 4$, $\hat{\theta} = 3$.


	\item 
	For two events $A_1$ and $A_2$, $A_1 \cap A_2$ is true if and only if $A_1$ is true and $A_2$ is true. When at least one of $A_1$ and $A_2$ is false then $A_1 \cap A_2$ is false. Then When both of them are true, $I(A_1) = I(A_2) = 1 $ and $I(A_1 \cap A_2) = 1 \Rightarrow I(A_1 \cap A_2) = I(A_1) I(A_2)$. When at least one of them is false, then $I(A_1) I(A_2) = 0$ and $I(A_1 \cap A_2) = 0$. Hence we have 
	\[I(A_1 \cap A_2) = I(A_1) I(A_2)\]
	Thus,
	\begin{align*}
	I(B) & = I(\bigcap_{i=1}^{n-1} A_i \cap A_n)\\
	& = I(\bigcap_{i=1}^{n-1} A_i) I(A_n)\\
	& = I(\bigcap_{i=1}^{n-2} A_i) I(A_{n-1})I(A_{n})\\
	& = \cdots\\
	& = \prod_{i=1}^n I(A_i)
	\end{align*}
	
	
	\item 
	\begin{enumerate}
		\item 
		$S_\theta = (0, + \infty)$ and $x_1, x_2, \cdots , x_n >0$, hence $I(x_1, x_2, \cdots , x_n \in S_\theta) = 1$. Then
		\[L(\theta) = \prod_{i=1}^n f(x_i | \theta) = \prod_{i=1}^n \frac{1}{\theta}\mathrm{e}^{-x_i / \theta} = \frac{1}{\theta^n} \mathrm{e}^{-\sum_{i=1}^n x_i / \theta} \]

		Then 
		\[\log L(\theta) = - n \log \theta - \frac{\sum_{i=1}^n x_i}{\theta}\]
		Let 
		\[\frac{\mathrm{d}}{\mathrm{d}\theta}\log L({\theta}) \bigg|_{\theta = \hat{\theta}} = 0 \Rightarrow - \frac{n}{\theta} + \frac{\sum_{i=1}^n x_i}{\theta^2} \bigg|_{\theta = \hat{\theta}} = 0 \Rightarrow \hat{\theta} = 	\frac{\sum_{i=1}^n X_i}{n} =  \bar{X}_n \]

		\item 
		$S_\theta = (0, \theta]$. As $x_1, x_2, \cdots, x_n >0$, then 
		$I(x_1, x_2, \cdots, x_n \in S_\theta) = I(x_1, x_2, \cdots, x_n \leq \theta) = I(\max_{1\leq i \leq n} x_i \leq \theta)$. Hence
		\begin{align*}
		L(\theta) & = \prod_{i=1}^n f(x_i | \theta) I(x_1, x_2, \cdots, x_n \in S_\theta)\\
		& = \prod_{i=1}^n \frac{2 x_i}{\theta^2} I(\max_{1 \leq i \leq n}x_i \leq \theta)\\
		& = \frac{2^n}{\theta^{2n}} \prod_{i=1}^n x_i I(\max_{1 \leq i \leq n}x_i \leq \theta) \\
		& = \begin{cases}
			\frac{2^n}{\theta^{2n}} \prod_{i=1}^n x_i & ,\theta \geq \max_{1 \leq i \leq n} x_i\\
			0 & , \theta < \max_{1 \leq i \leq n} x_i
		\end{cases}
				\end{align*}
		
		We can see $L(\max_{1 \leq i \leq n} x_i) > 0$ and $L(\theta)$ goes down as $\theta$ increasing when $\theta$ is greater than $\max_{1 \leq i \leq n} x_i$, thus it is the point when $L(\theta)$ is the largest. Hence
		\[\hat{\theta} = \max_{1 \leq i \leq n} X_i\]
	\end{enumerate}

	\item 
	\begin{enumerate}[start = 2]
		\item 
		$S_\theta = [\theta, \infty)$. Then 
		$I(x_1, x_2, \cdots, x_n \in S_\theta) = I(x_1, x_2, \cdots, x_n \geq \theta) = I(\min_{1\leq i \leq n} x_i \geq \theta)$. Hence
		\begin{align*}
		L(\theta) & = \prod_{i=1}^n f(x_i | \theta) I(x_1, x_2, \cdots, x_n \in S_\theta)\\
		& = \prod_{i=1}^n \theta x_i^{-2} I(\min_{1 \leq i \leq n}x_i \geq \theta)\\
		& = \theta^n (\prod_{i=1}^n x_i)^{-2} I(\min_{1 \leq i \leq n}x_i \geq \theta) \\
		& = \begin{cases}
			\theta^n (\prod_{i=1}^n x_i)^{-2} &, \theta \leq \min_{1 \leq i \leq n} x_i\\
			0 & , \theta > \min_{1 \leq i \leq n} x_i
		\end{cases}
				\end{align*}


		
		We can see $L(\min_{1 \leq i \leq n} x_i) > 0$ and $L(\theta)$ goes up as $\theta$ increasing when $\theta$ is less than $\min_{1 \leq i \leq n} x_i$, thus it is the point when $L(\theta)$ is the largest. Hence
		\[\hat{\theta} = \min_{1 \leq i \leq n} X_i\]


		\item 
		\[E(X) = \int_{\theta}^\infty x \theta x^{-2} \mathrm{d}x = \int_{\theta}^\infty \theta x^{-1} \mathrm{d}x = \theta \log x \bigg|_{\theta}^\infty = \infty\]

		Hence the MME does not exist.
	\end{enumerate}
	

	


 	\end{enumerate}


	
	
	
	\end{document}