
\documentclass{article}
\usepackage{amsmath,amssymb}
\usepackage[inline]{enumitem}
\usepackage{blindtext}
\usepackage{booktabs}
\usepackage{graphicx}
\usepackage{xcolor}
\usepackage[vmargin = 1.5in, top = 1in, bottom = 1.2in, letterpaper]{geometry}
\usepackage{listings}
\usepackage{courier}
\usepackage{multicol}
\usepackage{multirow}
\usepackage{bm}
\lstset{
basicstyle = \small\tt,
keywordstyle = \tt\color{blue},
commentstyle = \it\color[cmyk]{1,0,1,0},
stringstyle = \tt\color[RGB]{128,0,0},
%frame = single,
backgroundcolor = \color[RGB]{245,245,244},
breaklines,
extendedchars = false,
xleftmargin = 2em,
xrightmargin = 2em,
aboveskip = 1em,
tabsize = 4,
showspaces = false
}
\begin{document}
\setcounter{MaxMatrixCols}{20}

% \newfontfamily\courier{Courier New}


\title{STAT 510 Homework 7}
\author{Yifan Zhu}
\maketitle

\begin{enumerate}[leftmargin = 0 em, label = \arabic*., font = \bfseries]
	\item
	      \begin{enumerate}
	      	\item 
	      	\begin{align*}
	      	 E(MS_{ou(trt,xu)}) & = E \left(\frac{1}{tn(m-1)} \sum_{i=1}^t \sum_{j=1}^n \sum_{k = 1}^m (y_{ijk} - \bar{y}_{ij \cdot })^2 \right)\\
	      	 & = \frac{1}{tn(m-1)} E \left( \sum_{i=1}^t \sum_{j=1}^n \sum_{k=1}^m (\mu + \tau_i + u_{ij} + e_{ijk} - \mu - \tau_i - u_{ij} - \bar{e}_{ij \cdot})^2 \right) \\
	      	 & = \frac{1}{tn(m-1)} E \left( \sum_{i = 1}^t \sum_{j = 1}^n \sum_{k = 1}^m (e_{ijk} - \bar{e}_{ij \cdot} )^2 \right) \\
	      	 \end{align*}
	      	 As $e_ijk \sim N(0, \sigma_e^2)$, then
	      	 \begin{align*}
	      	 E \left( MS_{ou(trt, xu)} \right) & = \frac{1}{tn(m-1)} \sum_{i = 1}^r \sum_{j = 1}^n (m-1) \sigma_{e}^2\\
	      	 & = \frac{1}{tn (m-1)} tn (m-1) \sigma_e^2 \\
	      	 & = \sigma_e^2
	      	 \end{align*}
	      	 
	      	 \item 
	      	 Let $\bm A = (\bm I - \bm P_{3})$, where $\bm P_3 = \frac{1}{m} \bm I_{tn \times tn} \otimes \bm 1 \bm 1^T _{m \times m}$ is a projection matrix. Then $\bm y^T \bm A \bm y = \sum_{i=1}^t \sum_{j = 1}^n \sum_{k = 1}^m (y_{ijk} - \bar{y}_{ij \cdot})^2$. We also have 
	      	 \[ \Sigma = \sigma_u^2 \bm I_{tn \times tn} \otimes \bm 1 \bm 1^T_{m \times m} + \sigma_e^2 \bm I_{tnm \times tnm} = \sigma_{u}^2 m \bm P_{3} + \sigma_e^2 \bm I\]
	      	 Then

	      	 \begin{align*}
	      	 &\bm A \bm \Sigma = (\bm I - \bm P_3) (\sigma_u^2 m \bm P_3 + \sigma_e^2 \bm I) = \sigma_e^2 (\bm I - \bm P_3) = \sigma_e^2 (\bm I - \frac{1}{m} \bm I_{tn \times tn} \otimes \bm I_{m\times m})\\
	      	  \Rightarrow & \mathrm{tr}(\bm A \bm \Sigma) = tnm \sigma_e^2 (1 - \frac{1}{m}) = \sigma_e^2 tn (m-1)
	      	 \end{align*}

	      	 We know that $E(\bm y) \subset \mathcal{C}(\bm P_{2}) \subset \mathcal{C}(\bm P_{3})$. Thus $(\bm I - \bm P_{3}) E(\bm y) = \bm 0 \Rightarrow E(\bm y)^T \bm A E(\bm y) = 0$.
	      	 Hence,
	      	 \[E (\bm y^T \bm A \bm y) = tn(m-1) \sigma_e^2 \Rightarrow E(MS_{ou(trt, xu)}) = \frac{1}{tn(m-1)} tn (m-1) \sigma_e^2 = \sigma_e^2\]
	      	 


			  \end{enumerate}

			  \item 
			  \begin{enumerate}
			  	\item 
			  	$d_j = y_{1j} - y_{2j} = (\mu_1 + u _j + e_{1j}) - (\mu_2 + u_j + e_{2j}) = (\mu_1 - \mu_2) + (e_{1j} - e_{2j})$. We have $e_{ij} \overset{iid}{\sim} N(0, \sigma_{e}^2)$, then $d_j \overset{iid}{\sim} N(\mu_1 - \mu_2 , 2 \sigma_{e}^2)$.

			  	 \item 
			  	 \[T = \frac{\bar{d}}{\sqrt{\frac{1}{380} \sum_{j = 1}^{20} (d_j - \bar{d})^2}},\, \mathrm{where \ } \bar{d} = \frac{1}{20} \sum_{j = 1}^{20} d_j \] 


			  	 \item 
			  	 \[T \sim t_{19}(\mu_1 - \mu_2)\]

			  	 \item 
			  	 \[CI = \left[\bar{a} - \bar{b} - t_{38,0.975 }\sqrt{\frac{\sum_{j=1}^{20} (a_j - \bar{a})^2 + \sum_{j= 1}^2 (b_j - \bar{b})^2}{380}}, \bar{a} - \bar{b} + t_{38,0.975 }\sqrt{\frac{\sum_{j=1}^{20} (a_j - \bar{a})^2 + \sum_{j= 1}^2 (b_j - \bar{b})^2}{380}}\right]\]

			  	 \item 
			  	 \begin{align*}
			  	 & \hat{\sigma}_e^2 = \frac{\sum_{j = 1}^{20} (d_j - \bar{d})^2}{38}\\
			  	 & \hat{\sigma}_e^2 + \hat{\sigma}_u^2 = \frac{\sum_{j=1}^{20} (a_j - \bar{a})^2 + \sum_{j=1}^{20} (b_j - \bar{b})^2}{38} \Rightarrow \hat{\sigma}_u^2 = \frac{\sum_{j=1}^{20} (a_j - \bar{a})^2 + \sum_{j=1}^{20} (b_j - \bar{b})^2 - \sum_{j = 1}^{20} (d_j - \bar{d})^2}{38}
			  	 \end{align*}
			  	 
			  	 \item 
			  	 \begin{align*}
			  	 & \bm X = \begin{bmatrix}
			  	 	1 & -1\\
			  	 	\vdots & \vdots\\
			  	 	1 & -1\\
			  	 	1 & 0\\
			  	 	\vdots & \vdots\\
			  	 	1 & 0\\
			  	 	0 & 1\\
			  	 	\vdots & \vdots \\
			  	 	0 &ï¼‘
			  	 \end{bmatrix}\\
			  	 & \bm \Sigma = \begin{bmatrix}
			  	 	2 \sigma_e^2  \\
			  	 	& \ddots\\
			  	 	&& \sigma_e^2 \\
			  	 	&&& \sigma_e^2 + \sigma_u^2 \\
			  	 	&&&& \ddots \\
			  	 	&&&&& \sigma_e^2 + \sigma_u^2
			  	 \end{bmatrix}
			  	 \end{align*}
			  	 Then
			  	 \begin{align*}
			  	 \hat{\mu_1} - \hat{\mu_2} & = \begin{bmatrix}
			  	 	1 & -1
			  	 \end{bmatrix}
			  	 \bm (\bm X^T \bm \Sigma^{-1} \bm X)^- \bm X^T \bm \Sigma^{-1} \bm y \\
			  	 & = \frac{1}{\frac{1}{\sigma_e^2 + \sigma_u^2} + \frac{1}{\sigma_e^2}}\left(\frac{1}{\sigma_e^2} \bar{d} + \frac{1}{\sigma_u^2 + \sigma_e^2} (\bar{a} - \bar{b})\right)\\
			  	 & = \frac{1}{\sigma_{u}^2 + 2 \sigma_e^2} \left( (\sigma_u^2 + \sigma_e^2) \bar{d} + \sigma_e^2 (\bar{a} - \bar{b})\right)
			  	 \end{align*}
			  	 
			  	 
			  \end{enumerate}

			  \item 
			  \begin{align*}
			  & \bm X = \begin{bmatrix}
			  	\bm 1_{20 \times 1} \otimes \bm I_{2\times 2}\\
			  	\begin{bmatrix}
			  		\bm 1_{20 \times 1} & \bm 0_{20 \times 1}
			  	\end{bmatrix}\\
			  	\begin{bmatrix}
			  		\bm 0_{20 \times 1} & \bm 1_{20 \times 1}
			  	\end{bmatrix}
			  \end{bmatrix}\\
			  & \bm Z = \begin{bmatrix}
			  	\bm I_{20\times 20} \otimes \bm 1_{2\times 1} & \bm 0_{40\times 40}\\
			  	\bm 0_{40\times 20} & \bm I_{40\times 40}
			  \end{bmatrix}
			  \end{align*}

			  \item 
			  \begin{align*}
			  & \mathrm{BLUE}_1 (\mu) = \frac{y_1 + y_2 + y_3 + y_4}{4}\\
			  & \mathrm{Var}(\mathrm{BLUE}_1(\mu)) = \frac{1}{16} \mathrm{Var}(y_1 + y_2 + y_3 + y_4)\\
			  = & \frac{1}{16} \left(\sum_{i=1}^4 \mathrm{Var}(y_i) + \sum_{i \neq j} \mathrm{Cov}(y_i, y_j)\right)\\
			  =& \frac{1}{16}(5 \times 4 + 1 \times 4 \times 3) = 2 \\
			  & \mathrm{BLUE}_2(\mu) = y_5 \\
			  & \mathrm{Var}(\mathrm{BLUE}_2(\mu)) = \mathrm{Var}(y_5) = 4 
			  \end{align*}
			  We know $\mathrm{BLUE}_1(\mu)$ and $\mathrm{BLUE}_2 (\mu)$ are independent, then 
			  \[\mathrm{BLUE}(\mu) = \frac{\frac{1}{2}}{\frac{1}{2} + \frac{1}{4}} \mathrm{BLUE}_1(\mu) + \frac{\frac{1}{4}}{\frac{1}{2} + \frac{1}{4}} \mathrm{BLUE}_2 (\mu) = \frac{2}{3} \frac{y_1 + y_2 + y_3 + y_4}{4} + \frac{1}{3} y_5 = \frac{1}{6} (y_1 + y_2 + y_3 + y_4) + \frac{1}{3} y_5\]
			  
			  
			  
			   
	      \end{enumerate}
	      

\end{document}