
	\documentclass{article}
	\usepackage{amsmath,amssymb}
	\usepackage[inline]{enumitem}
	\usepackage{blindtext}
	\usepackage{booktabs}
	\usepackage{graphicx}
	\usepackage{xcolor}
	\usepackage[vmargin = 1.5in, top = 1in, bottom = 1.2in, letterpaper]{geometry}
	\usepackage{listings}
	\usepackage{courier}
	\usepackage{multicol}
	\usepackage{multirow}
	\usepackage{bm}
	\lstset{
	basicstyle = \small\tt,
	keywordstyle = \tt\color{blue},
	commentstyle = \it\color[cmyk]{1,0,1,0},
	stringstyle = \tt\color[RGB]{128,0,0},
	%frame = single,
	backgroundcolor = \color[RGB]{245,245,244},
	breaklines,
	extendedchars = false,
	xleftmargin = 2em,
	xrightmargin = 2em,
	aboveskip = 1em,
	tabsize = 4,
	showspaces = false
	}
	\begin{document}
	
	% \newfontfamily\courier{Courier New}

	
	\title{STAT 542 Homework 10}
	\author{Yifan Zhu}
	\maketitle
	
	\begin{enumerate}[leftmargin = 0 em, label = \arabic*., font = \bfseries]
	\item 
	$P(Y_i = 1) = P(X_i > \mu) = 1 - F_X (\mu),\, P(Y_i = 1) = P(X_i \leq \mu ) = F_X (\mu).$ Thus $Y_i \sim Bernolli(p = 1 - F_X (\mu))$. As $X_i$'s are iid, then $Y_i$'s are iid. Thus
	\[\sum_{i=1 }^n Y_i \sim Binomial(n, p = 1 - F_X (\mu))\]


	\item 
	Let $V = \sqrt{\frac{S^2 (n-1)}{\sigma^2}}$, then $V \sim \chi^2_{n-1}$. 

	\begin{align*}
	E(c \sqrt{S^2}) & = \frac{c \sigma}{\sqrt{n-1}}E\left(\sqrt{\frac{S^2 (n-1)}{\sigma^2}}\right)\\
	& = \frac{c \sigma}{\sqrt{n-1}} E(\sqrt{V})\\
	& = \frac{c \sigma}{\sqrt{n-1}} \int_{0}^\infty \sqrt{v}\frac{1}{\Gamma(\frac{n-1}{2}) 2^{\frac{n-1}{2}}} v^{\frac{n-1}{2} -1} \mathrm{e}^{- \frac{v}{2}} \mathrm{d}v\\
	& = \frac{c \sigma}{\sqrt{n-1}}  \frac{\Gamma{\frac{n}{2}} 2^{\frac{n}{2}}}{\Gamma(\frac{n-1}{2}) 2^{\frac{n-1}{2}}}\int_{0}^\infty \frac{1}{\Gamma(\frac{n}{2}) 2^{\frac{n}{2}}} v^{\frac{n}{2} - 1} \mathrm{e}^{- \frac{v}{2}} \mathrm{d}v\\
	& = c \frac{\sqrt{2} \Gamma(\frac{n}{2})}{\sqrt{n-1} \Gamma(\frac{n-1}{2})}
	\end{align*}

	Thus $E(c \sqrt{S^2}) = \sigma \Rightarrow c = \frac{\sqrt{n-1}\Gamma(\frac{n-1}{2})}{\sqrt{2} \Gamma(\frac{n}{2})}$ and $g(S^2) = \frac{\sqrt{n-1}\Gamma(\frac{n-1}{2})}{\sqrt{2} \Gamma(\frac{n}{2})} \sqrt{S^2}.$


	\item 
	\begin{enumerate}
		\item 
		$X_1 - 1, \frac{X_2 - 2}{2}, \frac{X_3 - 3}{3}$ are iid $N(0,1)$. then
		\[(X_1 -1)^2 + \left(\frac{X_2 - 2}{2}\right)^2 + \left(\frac{X_3 - 3}{3}\right)^2 \sim \chi^2_{3} \]


		\item 
		Let $Y_1 = X_1 - 1,\, Y_2 = \frac{X_2 - 2}{2},\, Y_3 = \frac{X_3 - 3}{3}, \bar{Y_3} = \frac{Y_1 + Y_2 + Y_3}{3} = \frac{1}{3}(X_1 + X_2/2 + X_3 /3) - 1, S = \sqrt{\frac{1}{2}\sum_{i = 1}^3 (Y_i - \bar{Y_3})^2}$ Then
		\[\frac{\sqrt{3} \bar{Y_3}}{S} \sim t_{2}\] 

		\item 
		\[\frac{3 \bar{Y_3}^2}{S^2} \sim F_{1,2}\]
	\end{enumerate}
	
	\item 
	$F_Z (z) = P(\min (X,Y) \leq z) = 1 - P(\min (X,Y) > z) = 1 - P(X>z)P(Y>z) = 1 - (1 - \Phi(z))^2$, then
	\begin{align*}
	F_{Z^2} (z) &= P(Z^2 \leq z)  = P(- \sqrt{z} \leq Z \leq \sqrt{z})\\
	& = F_{Z} (\sqrt{z}) - F_Z (-\sqrt{z})\\
	& = 1-(1 - \Phi(\sqrt{z}))^2 -1 + (1 - \Phi(-\sqrt{z}))^2\\
	& = -(1 - \Phi(\sqrt{z}))^2 + (\Phi (\sqrt{z}))^2\\
	& = 2 \Phi(\sqrt{z}) - 1
 	\end{align*}

 	Thus
 	\[f_{Z^2}(z) = \frac{\mathrm{d}}{\mathrm{d}z}F_{Z^2}(z) = \frac{1}{\sqrt{2 \pi}} \mathrm{e}^{-\frac{z}{2}} z^{-\frac{1}{2}}\]

 	Hence $Z^2 \sim \chi^2_{1}$


 	\item 
 	$f_X (x) = 1/\theta,\, F_X (x) = x/\theta,\, 0< x < \theta$.
 	\begin{align*}
 	f_{X_{(1)}, X_{(n)}}(u,v) & = \frac{n!}{0!(n-2)!0!} \frac{1}{\theta} \frac{1}{\theta} (\frac{u}{\theta})^0 (\frac{v - u}{\theta})^{n-2}(1 - \frac{v}{\theta})^0\\
 	& = \frac{n(n-1)}{\theta^n} (v - u)^{n-2},\quad 0< u< v <\theta
 	\end{align*}

 	Let $Z = \frac{X_{(1)}}{X_{(n)}},\, W = X_{(n)}$. Hence $X_{(1)} = ZW,\, X_{(n)} = W$, and
 	\[J = \begin{bmatrix}
 		w & z\\
 		0 & 1
 	\end{bmatrix},\, |\det J| = |w|\]

 	Thus

 	\begin{align*}
 	f_{Z,W} (z,w) & = \frac{n(n-1)}{\theta^n} (w - zw)^{n-2} w\\
 	& = \frac{n(n-1)}{\theta^n} (1 - z)^{n-2} w^{n-1},\quad 0<z<1, 0< w < \theta
 	\end{align*}

 	The support odf $(Z,W)$ is a rectangle, and $z$ and $w$ can be seperated, so they are independent.


 	\item 
 	\begin{enumerate}
 		\item 
 		$X$ and $Y$ are iid $N(0,1)$, thus $\begin{bmatrix}
 			X\\
 			Y
 		\end{bmatrix}$
 		is $MVN(\bm 0, I)$. Thus $\begin{bmatrix}
 			X\\
 			Z
 		\end{bmatrix}
 		=\begin{bmatrix}
 			X\\
 			X+Y
 		\end{bmatrix}
 		= \begin{bmatrix}
 			1&0\\
 			1&1
 		\end{bmatrix}
 		\begin{bmatrix}
 			X\\
 			Y
 		\end{bmatrix} $ . And $\bm \mu = \bm 0$ and $\Sigma  = \begin{bmatrix}
 			1&0\\
 			1&1
 		\end{bmatrix} 
 		\begin{bmatrix}
 			1&1\\
 			0&1
 		\end{bmatrix}=
 		\begin{bmatrix}
 			1&1\\
 			1&2
 		\end{bmatrix}$. Hence $\begin{bmatrix}
 			X\\
 			Z
 		\end{bmatrix} \sim MVN(\bm 0, \Sigma)$ 

 		\item 
 		For $\begin{bmatrix}
 			X - Y\\
 			X + Y
 		\end{bmatrix}$ we have
 		\[\begin{bmatrix}
 			X-Y\\
 			X+Y
 		\end{bmatrix} = \begin{bmatrix}
 			1 & -1\\
 			1 & 1
 		\end{bmatrix}
 		\begin{bmatrix}
 			X\\
 			Y
 		\end{bmatrix}.\] Thus $\begin{bmatrix}
 			X - Y\\
 			X+Y
 		\end{bmatrix} \sim MVN(\bm \mu, \Sigma)$, where $\bm \mu = \bm 0$ and $\Sigma = \begin{bmatrix}
 			1& -1\\
 			1 & 1
 		\end{bmatrix}
 		\begin{bmatrix}
 			1 & 1\\
 			-1 & 1
 		\end{bmatrix} = 
 		\begin{bmatrix}
 			2 & 0\\
 			0 & 2
 		\end{bmatrix}$. $\Sigma_{12} = \Sigma_{21} = 0$, thus $X-Y$ and $X+Y$ are independent. Then $g(x,y) = x-y$.

 		\item 
 		$F_{X|Z>0} (x) = \frac{P(X \leq x, Z >0)}{P(Z > 0)} = 2 \int_{-\infty}^x \int_{0}^{\infty} f(x,z) \mathrm{d}x \mathrm{d}z.$ Then $f_{X|Z>0} (x) = \frac{\mathrm{d}}{\mathrm{d}x} F_{X|Z>0}(x) = 2 \int_{0}^{\infty} f(x, z)\mathrm{d}z$. $\begin{bmatrix}
 		 			X & Z
 		 		\end{bmatrix}^{T}$ is $MVN$, then 

 		\[f(x,z) = \frac{1}{2 \pi} \mathrm{e}^{-\frac{1}{2}(2 x^2  - 2 z x + z^2)}\]
 		Thus
 		\begin{align*}
 		f_{X|Z>0}(x) & = 2 \frac{1}{2 \pi}\int_{0}^{\infty} \mathrm{e}^{-\frac{1}{2}(2x^2 - 2 zx + z^2)} \mathrm{d}z\\
 		& = \frac{\sqrt{2 \pi}}{\pi}\mathrm{e}^{-x^2 / 2} \int_{0}^\infty \frac{1}{\sqrt{2 \pi}}\mathrm{e}^{- (z - x)^2 / 2} \mathrm{d}z\\
 		& = \sqrt{\frac{2}{\pi}}\mathrm{e}^{-x^2 / 2} \int_{-x}^\infty \frac{1}{\sqrt{2 \pi}}\mathrm{e}^{- t^2 / 2} \mathrm{d}t\\
 		& = \sqrt{\frac{2}{\pi}}\mathrm{e}^{-x^2 / 2} (1 - \Phi (- x))\\
 		& = \sqrt{\frac{2}{\pi}}\mathrm{e}^{-x^2 / 2} \Phi(x)
 		\end{align*}
 		

 	\end{enumerate}

 	\item 
 	\begin{enumerate}
 		\item 
 		\begin{align*}
 	E[X] & = E[E[X|Y]] = E[Y] = \mu\\
 	Var[X] & = E[Var[X|Y]] + Var[E[X|Y]]\\
 	& = E[\sigma^2] + Var[Y]\\
 	& = \sigma^2 + \tau^2\\
 	E[XY] & = E[E[XY|Y]]\\
 	& = E[Y E[X|Y]]\\
 	& = E[Y^2]\\
 	& = Var[Y] + (E[Y])^2\\
 	& = \tau^2 + \mu^2\\
 	Cov(X,Y) & = E[XY] - E[X]E[Y]\\
 	& = \tau^2 + \mu^2 - \mu^2 = \tau^2
 	\end{align*}
 	
 	\item 
 	\[f(x,y) = f(x|y)f(y) = \frac{1}{\sqrt{2 \pi} \sigma} \mathrm{e}^{- \frac{(x - y)^2}{2 \sigma^2}} \frac{1}{\sqrt{2 \pi} \tau} \mathrm{e}^{- \frac{(y - \mu)^2}{2 \tau^2}} = \frac{1}{2 \pi \sigma \tau} \mathrm{e}^{-\frac{1}{2}((\frac{x - y}{\sigma})^2 + (\frac{y - \mu}{\tau})^2)}\]

 	From the variance of $[X,Y]^T$, we have $\Sigma = \begin{bmatrix}
 		\sigma^2 + \tau^2 & \tau^2\\
 		\tau^2 & \tau^2
 	\end{bmatrix}$ , $\det \Sigma = (\sigma^2 + \tau^2)\tau^2 - \tau^2 \cdot \tau^2 = \sigma^2 \tau^2$, and $\Sigma^{-1} = \begin{bmatrix}
 		1/\sigma^2 & - 1/\sigma^2\\
 		- 1 /\sigma^2 & 1/\sigma^2 + 1/\tau^2
 	\end{bmatrix}.$ Hence if $\begin{bmatrix}
 		X & Y
 	\end{bmatrix}^T$ is $MVN$, then
 	\begin{align*}
 	f(x,y)& = \left(\frac{1}{(2 \pi)^2 \det \Sigma}\right)^{1/2} \mathrm{e}^{- \frac{1}{2}\begin{bmatrix}
 		x - \mu & y - \mu
 	\end{bmatrix} \Sigma^{-1} \begin{bmatrix}
 		x - \mu\\
 		y - \mu
 	\end{bmatrix}}\\
 	& = \frac{1}{2 \pi \sigma \tau} \mathrm{e}^{-\frac{1}{2} ((\frac{x - \mu}{\sigma})^2 - \frac{(y - \mu)(x - \mu)}{\sigma^2} - \frac{(x - \mu)(y - \mu)}{\sigma^2} + (\frac{y - \mu}{\sigma})^2 + (\frac{y - \mu}{\tau})^2)}\\
 	& = \frac{1}{2 \pi \sigma \tau} \mathrm{e}^{-\frac{1}{2}((\frac{x - y}{\sigma})^2 + (\frac{y - \mu}{\tau})^2)}
 	\end{align*}
 	It is the same as what we get from the conditional density, thus $\begin{bmatrix}
 		X & Y
 	\end{bmatrix}^T \sim MVN(\bm \mu, \Sigma)$.
 	\end{enumerate}
 	
 	
 	
 	
 	
	
	
 	\end{enumerate}






	
	\end{document}