
	\documentclass{article}
	\usepackage{amsmath,amssymb}
	\usepackage{enumitem}
	\usepackage{blindtext}
	\usepackage{booktabs}
	\usepackage{graphicx}
	\usepackage{xcolor}
	\usepackage[vmargin = 1.5in, top = 1in, bottom = 1.2in, letterpaper]{geometry}
	\usepackage{listings}
	\usepackage{courier}
	\lstset{
	basicstyle = \small\tt,
	keywordstyle = \tt\color{blue},
	commentstyle = \it\color[cmyk]{1,0,1,0},
	stringstyle = \tt\color[RGB]{128,0,0},
	%frame = single,
	backgroundcolor = \color[RGB]{245,245,244},
	breaklines,
	extendedchars = false,
	xleftmargin = 2em,
	xrightmargin = 2em,
	aboveskip = 1em,
	tabsize = 4,
	showspaces = false
	}
	\begin{document}
	
	% \newfontfamily\courier{Courier New}

	
	\title{STAT 542 Homework 3}
	\author{Yifan Zhu}
	\maketitle
	
	\begin{enumerate}[leftmargin = 0 em, label = \arabic*., font = \bfseries]
	\item Support of $f_Y$ is $\mathcal{Y} = \{\frac{k}{k+1}|k = 0, 1, 2, \cdots\}$. 

	$P(Y = y) = P(\frac{X}{X+1} = y) = P(X = \frac{y}{1 - y}) = \frac{1}{3} (\frac{2}{3})^{y/(1-y)},\, y = 0, \frac{1}{2}, \frac{2}{3}, \frac{3}{4} \cdots$.

	Thus, pmf of $Y$ 
	\[f_Y (y) = \begin{cases}
	\frac{1}{3} (\frac{2}{3})^{y/(1-y)} & y = 0, \frac{1}{2}, \frac{2}{3}, \frac{3}{4} \cdots\\
	0 & \mathrm{otherwise}
	\end{cases}\]
	
	\item \begin{enumerate}
		\item 
	\begin{align*}
	&\int_{-\infty}^{\infty} f(x) \mathrm{d}x \\
	=& \int_{-\infty}^0 \frac{1}{2} \lambda \mathrm{e}^{\lambda x} \mathrm{d}x + \int_{0}^{\infty} \frac{1}{2} \lambda \mathrm{e}^{- \lambda x}\mathrm{d}x\\
	=& \left. \frac{1}{2} \mathrm{e}^{\lambda x}\right|_{-\infty}^0 -   \left. \frac{1}{2} \mathrm{e}^{-\lambda x}\right|_{0}^\infty\\
	= & \frac{1}{2} - (- \frac{1}{2}) = 1
	\end{align*}
$f(x) \geq 0$ for $x \in \mathbb{R}$ and the integral is 1, thus $f(x)$ is a cdf.

\item For $t \leq 0$, 
\begin{align*}
P(X < t) & = \int_{-\infty}^0 f(x) \mathrm{d}x\\
& = \int_{-\infty}^t \frac{1}{2}\lambda \mathrm{e}^{\lambda x} \mathrm{d}x\\
& = \left.\frac{1}{2} \mathrm{e}^{\lambda x} \right|_{-\infty}^t  = \frac{1}{2} \mathrm{e}^{\lambda t}
\end{align*}
For $t > 0$,
\begin{align*}
P(X < t ) & = \int_{-\infty}^{t} f(x) \mathrm{d}x\\
& = \int_{-\infty}^0 \frac{1}{2} \lambda \mathrm{e}^{\lambda x} \mathrm{d}x + \int_{0}^{t} \frac{1}{2} \lambda \mathrm{e}^{- \lambda x} \mathrm{d}x\\
& = \frac{1}{2} -\left. \frac{1}{2} \mathrm{e}^{-\lambda x}\right|_{0}^t\\
& = 1 - \left(\frac{1}{2} \mathrm{e}^{-\lambda t} - \frac{1}{2}\right) = 1 - \frac{1}{2} \mathrm{e}^{- \lambda t}
\end{align*}
Thus
\[P(X < t) = \begin{cases}
\frac{1}{2} \mathrm{e}^{\lambda t} & t \leq 0\\
1 - \frac{1}{2} \mathrm{e}^{- \lambda t} & t > 0
\end{cases}\]

\item 
For $t \geq 0$
\begin{align*}
P(|X| < t) &= P(-t < X < t) = \int_{-t}^0 \frac{1}{2} \lambda \mathrm{e}^{\lambda x} \mathrm{d}x + \int_{0}^\infty \frac{1}{2} \lambda \mathrm{e}^{-\lambda x} \mathrm{d} x \\
&=\left.\frac{1}{2} \mathrm{e}^{\lambda x} \right|_{-t}^0 - \left.\frac{1}{2} \mathrm{e}^{\lambda x} \right|_{0}^t\\
&= \frac{1}{2} - \frac{1}{2} \mathrm{e}^{- \lambda t} - \left(\frac{1}{2} \mathrm{e}^{-\lambda t} - \frac{1}{2}\right)\\
& = 1 - \mathrm{e}^{-\lambda t}
 \end{align*}
 For $t < 0$, $P(|X| < t) = 0$. Thus
 \[P(|X| < t) = \begin{cases}
 0 & t <0\\
 1 - \mathrm{e}^{- \lambda t} & t \geq 0
 \end{cases}\]

\end{enumerate}

\item \begin{enumerate}[start = 2]
	\item Let $A_1 = (-1,0],\, A_2 = (0,1). \, g_1 (x) = 1- x^2,\, g_1^{-1}(y) = -\sqrt{1 - y}.\, g_2 (x) = 1 - x^2,\, g_2^{-1} (y) = \sqrt{1 - y}$. $g_1$ and $g_2$ are monotone on $A_1$ and $A_2$, thus
	\begin{align*}
	f_Y(y) &= f_X(g_1^{-1}(y))|{g_1^{-1}}'(y)| +  f_X(g_2^{-1}(y))|{g_2^{-1}}'(y)|\\
	& = \frac{3}{8} (1 - \sqrt{1 - y})^2 \frac{1}{2 \sqrt{1 - y}} + \frac{3}{8} (1 + \sqrt{1 - y})^2 \frac{1}{2 \sqrt{1 - y}}\\
	& = \frac{3}{8} \frac{2 - y}{\sqrt{1 - y}}
	\end{align*}

	\item  Let $A_1 = (-1,0],\, A_2 = (0,1). \, g_1 (x) = 1- x^2,\, g_1^{-1}(y) = -\sqrt{1 - y}.\, g_2 (x) = 1 - x,\, g_2^{-1} (y) = 1 - y$. $g_1$ and $g_2$ are monotone on $A_1$ and $A_2$, thus
	\begin{align*}
	f_Y(y) &= f_X(g_1^{-1}(y))|{g_1^{-1}}'(y)| +  f_X(g_2^{-1}(y))|{g_2^{-1}}'(y)|\\
	& = \frac{3}{8} (1 - \sqrt{1 - y})^2 \frac{1}{2 \sqrt{1 - y}} + \frac{3}{8} (1 + 1 - y)^2 |-1|\\
	& = \frac{3}{16}(1 - \sqrt{1- y})^2 \frac{1}{\sqrt{1 - y}}+ \frac{3}{8} (2 - y)^2
	\end{align*}
	
\end{enumerate}

\item The cdf of $X$ is 
\[F_X (x) = \begin{cases}
0 & x <1\\
\frac{1}{4} (x -1)^2 & 1 \leq x \leq 3\\
1 & x>3
\end{cases}\]

Let $Y = u(X) = F_X (X) $. Then for $y\leq 0, $
\[P(Y\leq y) = P(Y = 0) = P(X \leq 1) = F_{X}(1) = 0 \]
For $0 <  y \leq 1 $,
\[P(Y \leq y) = P(X\leq 2 \sqrt{y}+1) = F_{X}(2 \sqrt{y} +1) = y\]
For $y > 1$,
\[P(Y\leq y) = 1\]
Thus the cdf of $Y$ is
\[F_Y(y) = \begin{cases}
0 & y\leq 0\\
y & 0<y\leq 1\\
1 & y > 1
\end{cases}\]
Hence, $Y \sim \mathrm{unif}(0,1)$.

\item \begin{enumerate}
	\item Let $y = \frac{\beta}{\sqrt{2}}y$. Then
	\begin{align*}
	\int_{-\infty}^\infty f(x) \mathrm{d}x &= \int_{0}^\infty \frac{4}{\beta^3 \sqrt{\pi}}x^2 \mathrm{e}^{-x^2 / \beta^2}  \mathrm{d}x\\
	&= \int_{0}^\infty \frac{4}{\beta^3 \sqrt{\pi}} \frac{\beta^2}{2}y^2 \mathrm{e}^{-y^2 /2}\frac{\beta}{\sqrt{2}} \mathrm{d}y\\
	& = \frac{2}{\sqrt{2 \pi}} \int_{0}^\infty y^2 \mathrm{e}^{- y^2 / 2} \mathrm{d}y = 1
	\end{align*}
	The integral is 1 and $f(x) \geq 0$ for $x\in \mathbb{R}$, thus $f(x)$ is a pdf.
	
	\item Let $y = \frac{\beta}{\sqrt{2}}y$. Then
	\begin{align*}
	E(X) = \int_{-\infty}^\infty x f(x) \mathrm{d}x &= \int_{0}^\infty \frac{4}{\beta^3 \sqrt{\pi}}x^3 \mathrm{e}^{-x^2 / \beta^2}  \mathrm{d}x\\
	 &= \int_{0}^\infty \frac{4}{\beta^3 \sqrt{\pi}} \frac{\beta^3}{2\sqrt{2}}y^2 \mathrm{e}^{-y^2 /2}\frac{\beta}{\sqrt{2}} \mathrm{d}y\\
	& = \frac{\beta}{\sqrt{\pi}} \int_{0}^\infty y^3 \mathrm{e}^{- y^2 / 2} \mathrm{d}y\\
	&= \frac{\beta}{\sqrt{\pi}} \int_{0}^\infty y^2 \mathrm{d}\left(- \mathrm{e}^{-y^2 /2}\right)\\
	&= \frac{\beta}{\sqrt{\pi}} \left[ \left.-y^2 \mathrm{e}^{-y^2 /2}\right|_{0}^\infty + \int_{0}^{\infty} \mathrm{e}^{-y^2 /2}\mathrm{d}{y^2}\right]\\
	& = \frac{\beta}{\sqrt{\pi}}\int_{0}^{\infty} \mathrm{e}^{-t/2}\mathrm{d}t = \left.-2\mathrm{e^{-t/2}}\right|_{0}^\infty = \frac{\beta}{\sqrt{\pi}} \cdot 2 = \frac{2 \beta }{\sqrt{\pi}}
	\end{align*}

	In the second last line, $\lim_{y\to \infty} y^2 \mathrm{e}^{-y^2 /2} = 0$
\end{enumerate}

\item \begin{align*}
E(Y) &= EX^2 = \int_{-\infty}^\infty x^2 f(x) \mathrm{d}x\\
&= \int_{-1}^1 \frac{1}{2} x^2(1+x) \mathrm{d}x\\
& = \left.\frac{1}{6} x^3 + \frac{1}{8}x^4 \right|_{-1}^{1}\\
& = \frac{1}{3}
\end{align*}
\begin{align*}
E(Y^2) &= E(X^4) = \int_{-\infty}^\infty x^4 f(x) \mathrm{d}x\\
&=\int_{-1}^1 \frac{1}{2}x^4(1+x)\mathrm{d}x\\
&= \left. \frac{1}{10}x^5 + \frac{1}{12}x^6 \right|_{-1}^1\\
&=\frac{1}{5}\\
Var(Y) &= E(Y^2) - (EY)^2 = \frac{1}{5} - (\frac{1}{3})^2 = \frac{4}{45}
\end{align*}

\item \begin{enumerate}
	\item \[P(X = x ) =\begin{cases}
	 (\frac{1}{2})^{x-1}\frac{1}{2} = (\frac{1}{2})^x & x = 1,2,3,\cdots\\
	 0 & \mathrm{otherwise}
	 \end{cases}\]


	 \item $X \sim \mathrm{Geometric}(\frac{1}{2})$, thus $EX = \frac{1}{1/2} = 2$.

	 \item $X_m = X-1,\, X_f = 1.$ Thus $E(X_m) = E(X-1) = EX -1 = 1,\, E(X_f) = 1 $.

\end{enumerate}

\item \begin{enumerate}
	\item $F_Y(y) = P(Y\leq y) = P(F^{-1}(U)\leq y)=P(U\leq F(y)) = F(y).$ (bacause $0\leq F(y) \leq 1$) Thus $Y$ and $X$ have the same distribution.

	\item For $u > 0$, cdf of $Z$
	\begin{align*}
	F_Z(u) &= \int_{0}^u f_Z (z) \mathrm{d}z = \int_{0}^u 2z e^{-z^2}\mathrm{d}z\\
	&= \int_{0}^u \mathrm{e}^{-z^2}\mathrm{d}z^2 = \int_{0}^u^2 \mathrm{e}^{-t}\mathrm{d}t\\
	& =\left.-\mathrm{e}^{-t}\right|_{0}^{u^2}\\
	&= 1 - \mathrm{e}^{-u^2}
	\end{align*}
	On $(0,\infty)$, we have $F_Z: (0,\infty)\mapsto (0,1)$ and it is monotone.So the inverse $F_Z^{-1}: (0,1)\mapsto (0,\infty)$.
	$F_Z^{-1}(u) = \sqrt{-\log (1-u)}$. Let $Z = \sqrt{-\log (1-U)} $ , where $U \sim \mathrm{unif}(0,1)$, then $Z$ distributes according to $f_Z$. With the randonly generated numbers distributed unifornly on $(0,1)$, we can plugin these numbers into $\sqrt{-\log (1- (\cdot))}$ to get the numbers distributed according to $f_Z$.  
\end{enumerate}


 	\end{enumerate}


	
	
	
	\end{document}